Adapt PCUIC to new projection invariant

pcuic/theories/PCUICClosed.v
@@ -17,6 +17,32 @@ Definition closedn_ctx n ctx :=
 
 Notation closed_ctx ctx := (closedn_ctx 0 ctx).
 
+Lemma lift_decl_closed n k d : closed_decl k d -> lift_decl n k d = d.
+Proof.
+  case: d => na [body|] ty; rewrite /closed_decl /lift_decl /map_decl /=.
+  - move/andP => [cb cty]. now rewrite !lift_closed //.
+  - move=> cty; now rewrite !lift_closed //.
+Qed.
+
+Lemma closed_decl_upwards k d : closed_decl k d -> forall k', k <= k' -> closed_decl k' d.
+Proof.
+  case: d => na [body|] ty; rewrite /closed_decl /=.
+  - move/andP => [cb cty] k' lek'. do 2 rewrite (@closed_upwards k) //.
+  - move=> cty k' lek'; rewrite (@closed_upwards k) //.
+Qed.
+
+Lemma closed_ctx_lift n k ctx : closedn_ctx k ctx -> lift_context n k ctx = ctx.
+Proof.
+  induction ctx in n, k |- *; auto.
+  unfold closed_ctx, id. rewrite lift_context_snoc.
+  simpl.
+  rewrite /mapi mapi_rec_app forallb_app List.rev_length /= /snoc Nat.add_0_r.
+  move/andb_and => /= [Hctx /andb_and [Ha _]].
+  f_equal. rewrite lift_decl_closed. apply: closed_decl_upwards; eauto. lia. 
+  reflexivity.
+  rewrite IHctx // lift_decl_closed //. 
+Qed.
+
 Lemma map_decl_ext' f g k d : closed_decl k d -> 
   (forall x, closedn k x -> f x = g x) -> 
   map_decl f d = map_decl g d.
@@ -291,33 +317,6 @@ Proof.
   f_equal. lia.
 Qed.
 
-Lemma lift_decl_closed n k d : closed_decl k d -> lift_decl n k d = d.
-Proof.
-  case: d => na [body|] ty; rewrite /closed_decl /lift_decl /map_decl /=.
-  - move/andP => [cb cty]. now rewrite !lift_closed //.
-  - move=> cty; now rewrite !lift_closed //.
-Qed.
-
-Lemma closed_decl_upwards k d : closed_decl k d -> forall k', k <= k' -> closed_decl k' d.
-Proof.
-  case: d => na [body|] ty; rewrite /closed_decl /=.
-  - move/andP => [cb cty] k' lek'. do 2 rewrite (@closed_upwards k) //.
-  - move=> cty k' lek'; rewrite (@closed_upwards k) //.
-Qed.
-
-
-Lemma closed_ctx_lift n k ctx : closedn_ctx k ctx -> lift_context n k ctx = ctx.
-Proof.
-  induction ctx in n, k |- *; auto.
-  unfold closed_ctx, id. rewrite lift_context_snoc.
-  simpl.
-  rewrite /mapi mapi_rec_app forallb_app List.rev_length /= /snoc Nat.add_0_r.
-  move/andb_and => /= [Hctx /andb_and [Ha _]].
-  f_equal. rewrite lift_decl_closed. apply: closed_decl_upwards; eauto. lia. 
-  reflexivity.
-  rewrite IHctx // lift_decl_closed //. 
-Qed.
-
 Lemma closedn_mkProd_or_LetIn (Γ : context) d T :
     closed_decl #|Γ| d ->
     closedn (S #|Γ|) T -> closedn #|Γ| (mkProd_or_LetIn d T).
@@ -364,15 +363,193 @@ Proof.
       now rewrite app_length // plus_n_Sm.
 Qed.
 
+Lemma type_local_ctx_All_local_env {cf:checker_flags} P Σ Γ Δ s : 
+  All_local_env (lift_typing P Σ) Γ ->
+  type_local_ctx (lift_typing P) Σ Γ Δ s ->
+  All_local_env (lift_typing P Σ) (Γ ,,, Δ).
+Proof.
+  induction Δ; simpl; auto.
+  destruct a as [na [b|] ty];
+  intros wfΓ wfctx; constructor; intuition auto.
+   exists s; auto.
+Qed.
+
+Definition Pclosed :=
+  (fun (_ : global_env_ext) (Γ : context) (t T : term) =>
+           closedn #|Γ| t && closedn #|Γ| T).
+
+Lemma type_local_ctx_Pclosed Σ Γ Δ s :
+  type_local_ctx (lift_typing Pclosed) Σ Γ Δ s ->
+  Alli (fun i d => closed_decl (#|Γ| + i) d) 0 (List.rev Δ).
+Proof.
+  induction Δ; simpl; auto; try constructor.  
+  destruct a as [? [] ?]; intuition auto.
+  - apply Alli_app_inv; auto. constructor. simpl.
+    rewrite List.rev_length. 2:constructor.
+    unfold closed_decl. unfold Pclosed in b0. simpl.
+    rewrite app_context_length in b0. now rewrite Nat.add_comm.
+  - apply Alli_app_inv; auto. constructor. simpl.
+    rewrite List.rev_length. 2:constructor.
+    unfold closed_decl. unfold Pclosed in b. simpl.
+    rewrite app_context_length in b. rewrite Nat.add_comm.
+    now rewrite andb_true_r in b.
+Qed.
+
+Lemma All_local_env_Pclosed Σ Γ :
+  All_local_env ( lift_typing Pclosed Σ) Γ ->
+  Alli (fun i d => closed_decl i d) 0 (List.rev Γ).
+Proof.
+  induction Γ; simpl; auto; try constructor.  
+  intros all; depelim all; intuition auto.
+  - apply Alli_app_inv; auto. constructor. simpl.
+    rewrite List.rev_length. 2:constructor.
+    unfold closed_decl. unfold Pclosed in l. simpl. red in l.
+    destruct l as [s H].
+    now rewrite andb_true_r in H.
+  - apply Alli_app_inv; auto. constructor. simpl.
+    rewrite List.rev_length. 2:constructor.
+    unfold closed_decl. unfold Pclosed, lift_typing in *. now simpl.
+Qed.
+
+Lemma closed_subst_context (Γ Δ Δ' : context) t :
+  closedn (#|Γ| + #|Δ|) t ->
+  Alli (fun i d => closed_decl (#|Γ| + S #|Δ| + i) d) 0 (List.rev Δ') -> 
+  Alli (fun i d => closed_decl (#|Γ| + #|Δ| + i) d) 0 (List.rev (subst_context [t] 0 Δ')).
+Proof.
+  induction Δ' in Δ |- *.
+  intros. simpl. auto. constructor.
+  destruct a as [? [] ?]; simpl.
+  - intros. eapply Alli_app in X as [X X'].
+    rewrite subst_context_snoc. simpl. eapply Alli_app_inv.
+    eapply IHΔ'; eauto. constructor; [|constructor].
+    simpl. 
+    rewrite /closed_decl /map_decl /= Nat.add_0_r List.rev_length subst_context_length.
+    inv X'. unfold closed_decl in H0. simpl in H0.
+    rewrite List.rev_length Nat.add_0_r in H0.
+    move/andP: H0 => [Hl Hr].
+    rewrite !closedn_subst /= ?H //; eapply closed_upwards; eauto; try lia.
+  - intros. eapply Alli_app in X as [X X'].
+    rewrite subst_context_snoc. simpl. eapply Alli_app_inv.
+    eapply IHΔ'; eauto. constructor; [|constructor].
+    simpl. 
+    rewrite /closed_decl /map_decl /= Nat.add_0_r List.rev_length subst_context_length.
+    inv X'. unfold closed_decl in H0. simpl in H0.
+    rewrite List.rev_length Nat.add_0_r in H0.
+    rewrite !closedn_subst /= ?H //; eapply closed_upwards; eauto; try lia.
+Qed.
+
+Lemma closed_smash_context_gen (Γ Δ Δ' : context) :
+  Alli (fun i d => closed_decl (#|Γ| + i) d) 0 (List.rev Δ) -> 
+  Alli (fun i d => closed_decl (#|Γ| + #|Δ| + i) d) 0 (List.rev Δ') -> 
+  Alli (fun i d => closed_decl (#|Γ| + i) d) 0 (List.rev (smash_context Δ' Δ)).
+Proof.
+  induction Δ in Δ' |- *.
+  intros. simpl. auto.
+  simpl. eapply (Alli_impl _ X0). simpl. now rewrite Nat.add_0_r.
+  destruct a as [? [] ?]; simpl.
+  - intros. eapply Alli_app in X as [X X'].
+    eapply IHΔ; eauto.
+    inv X'. unfold closed_decl in H. simpl in H.
+    rewrite List.rev_length Nat.add_0_r in H.
+    clear X1. eapply closed_subst_context; auto.
+    now move/andP: H => [].
+  - intros. eapply Alli_app in X as [X X'].
+    eapply IHΔ; eauto.
+    inv X'. unfold closed_decl in H. simpl in H.
+    rewrite List.rev_length Nat.add_0_r in H.
+    clear X1. rewrite List.rev_app_distr.
+    eapply Alli_app_inv; repeat constructor.
+    now rewrite /closed_decl Nat.add_0_r /=.
+    rewrite List.rev_length /=. clear -X0.
+    apply Alli_shift, (Alli_impl _ X0). intros.
+    eapply closed_decl_upwards; eauto; lia.
+Qed.
+
+Lemma closed_smash_context (Γ Δ : context) :
+  Alli (fun i d => closed_decl (#|Γ| + i) d) 0 (List.rev Δ) -> 
+  Alli (fun i d => closed_decl (#|Γ| + i) d) 0 (List.rev (smash_context [] Δ)).
+Proof.
+  intros; apply (closed_smash_context_gen Γ _ []); auto. constructor.
+Qed.
+
+Lemma context_assumptions_app Γ Δ : context_assumptions (Γ ++ Δ) = 
+  context_assumptions Γ + context_assumptions Δ.
+Proof.
+  induction Γ as [|[? [] ?] ?]; simpl; auto.
+Qed.
+
+Lemma weaken_env_prop_closed {cf:checker_flags} : 
+  weaken_env_prop (lift_typing (fun (_ : global_env_ext) (Γ : context) (t T : term) =>
+  closedn #|Γ| t && closedn #|Γ| T)).
+Proof. repeat red. intros. destruct t; red in X0; eauto. Qed.
+
+Lemma declared_projection_closed_ind {cf:checker_flags} {Σ : global_env_ext} {mdecl idecl p pdecl} : 
+  wf Σ.1 ->
+  declared_projection Σ.1 mdecl idecl p pdecl ->
+  Forall_decls_typing
+  (fun _ (Γ : context) (t T : term) =>
+  closedn #|Γ| t && closedn #|Γ| T) Σ.1 ->
+  closedn (S (ind_npars mdecl)) pdecl.2.
+Proof.
+  intros wfΣ isdecl X0.
+  pose proof (declared_projection_inv weaken_env_prop_closed wfΣ X0 isdecl) as onp.
+  set (declared_inductive_inv _ wfΣ X0 isdecl.p1) as oib in *.
+  clearbody oib.
+  have onpars := onParams _ _ _ _ (declared_minductive_inv weaken_env_prop_closed wfΣ X0 isdecl.p1.p1).
+  have parslen := onNpars _ _ _ _ (declared_minductive_inv weaken_env_prop_closed wfΣ X0 isdecl.p1.p1).
+  simpl in onp. destruct (ind_cshapes oib) as [|? []] eqn:Heq; try contradiction.
+  red in onp.
+  destruct (nth_error (smash_context [] _) _) eqn:Heq'; try contradiction.
+  rewrite {}onp. 
+  pose proof (onConstructors oib) as onc. 
+  red in onc. rewrite Heq in onc. inv onc. clear X1.
+  eapply on_cargs in X.
+  simpl.
+  replace (S (ind_npars mdecl)) with (0 + (1 + ind_npars mdecl)) by lia.
+  eapply closedn_subst.
+  { clear. unfold inds. generalize (ind_bodies mdecl).
+    induction l; simpl; auto. }
+  rewrite inds_length.
+  eapply closedn_subst0.
+  { clear. unfold projs. induction p.2; simpl; auto. }
+  rewrite projs_length /=.
+  eapply (@closed_upwards (ind_npars mdecl + #|ind_bodies mdecl| + p.2 + 1)).
+  2:lia.
+  eapply closedn_lift.
+  clear -parslen isdecl Heq' onpars X.
+  rename X into args.
+  apply type_local_ctx_Pclosed in args.
+  red in onpars.
+  eapply All_local_env_Pclosed in onpars.
+  eapply (Alli_impl (Q:=fun i d => closed_decl (#|ind_params mdecl| + i + #|arities_context (ind_bodies mdecl)|) d)) in args.
+  2:{ intros n x. rewrite app_context_length. 
+      intros H; eapply closed_decl_upwards; eauto. lia. }
+  eapply (Alli_shiftn (P:=fun i d => closed_decl (i + #|arities_context (ind_bodies mdecl)|) d)) in args.
+  rewrite Nat.add_0_r in args.
+  eapply (Alli_impl (Q:=fun i d => closed_decl (i + #|arities_context (ind_bodies mdecl)|) d)) in onpars.
+  2:{ intros n x d. eapply closed_decl_upwards; eauto; lia. }
+  epose proof (Alli_app_inv onpars). rewrite List.rev_length /= in X.
+  specialize (X args). rewrite -List.rev_app_distr in X.
+  clear onpars args.
+  eapply (Alli_impl (Q:=fun i d => closed_decl (#|arities_context (ind_bodies mdecl)| + i) d)) in X.
+  2:intros; eapply closed_decl_upwards; eauto; lia.
+  eapply closed_smash_context in X.
+  eapply Alli_rev_nth_error in X; eauto.
+  rewrite smash_context_length in X. simpl in X.
+  eapply nth_error_Some_length in Heq'. rewrite smash_context_length in Heq'.
+  simpl in Heq'. unfold closed_decl in X.
+  move/andP: X => [] _ cl.
+  eapply closed_upwards. eauto. rewrite arities_context_length.
+  rewrite context_assumptions_app parslen.
+  rewrite context_assumptions_app in Heq'. lia.
+Qed.
+
 Lemma typecheck_closed `{cf : checker_flags} :
   env_prop (fun Σ Γ t T =>
               closedn #|Γ| t && closedn #|Γ| T)
-            (fun Σ Γ _ => closed_ctx Γ).
+           (fun Σ Γ _ => closed_ctx Γ).
 Proof.
-  assert(weaken_env_prop (lift_typing (fun (_ : global_env_ext) (Γ : context) (t T : term) =>
-                                         closedn #|Γ| t && closedn #|Γ| T))).
-  { repeat red. intros. destruct t; red in X0; eauto. }
-
+  assert (X := weaken_env_prop_closed).
   apply typing_ind_env; intros * wfΣ Γ wfΓ *; simpl; intros; rewrite -> ?andb_and in *; try solve [intuition auto].
 
   - induction X0; simpl; auto; rewrite (closedn_ctx_app _ Γ [_]); simpl.
@@ -431,10 +608,9 @@ Proof.
       pose proof X0.(onConstructors) as XX.
       eapply All2_nth_error_Some in Hcdecl; eauto.
       destruct Hcdecl as [? [? ?]]. cbn in *.
-      destruct o as [? [s Hs] _]. rewrite -> andb_and in Hs.
+      destruct o as [? ? ? [s Hs] _]. rewrite -> andb_and in Hs.
       apply proj1 in Hs.
-      unfold arities_context in Hs.
-      rewrite rev_map_length in Hs.
+      rewrite arities_context_length in Hs.
       eauto using closed_upwards with arith.
 
   - intuition auto.
@@ -450,19 +626,9 @@ Proof.
     + simpl. apply closedn_mkApps_inv in H3.
       rewrite forallb_rev H2. apply H3.
     + rewrite closedn_subst_instance_constr.
-      eapply declared_projection_inv in isdecl as H'; eauto.
-      apply on_declared_projection in isdecl as [[Hmdecl Hidecl] Hpdecl]; auto.
-      red in Hpdecl.
-      destruct Hpdecl as [s Hs]. simpl in *.
-      apply onNpars in Hmdecl.
-      cbn in H'; destruct H'.
-      simpl in *.
-      rewrite List.rev_length H1.
-      rewrite andb_true_r in i. rewrite <- Hmdecl.
-      rewrite smash_context_length in i. simpl in i.
-      eapply closed_upwards; eauto.
-      change PCUICEnvironment.context_assumptions with context_assumptions.
-      lia.
+      eapply declared_projection_closed_ind in X0; eauto.
+      simpl; rewrite List.rev_length H1.
+      eapply closed_upwards; eauto. lia.
 
   - clear H.
     split. solve_all.
@@ -513,7 +679,7 @@ Proof.
     -- eapply Alli_impl. exact onI. eauto. intros.
        refine {| ind_indices := X1.(ind_indices);
                  ind_arity_eq := X1.(ind_arity_eq);
-                 ind_ctors_sort := X1.(ind_ctors_sort) |}.
+                 ind_cshapes := X1.(ind_cshapes) |}.
        --- apply onArity in X1. unfold on_type in *; simpl in *.
            now eapply X.
        --- pose proof X1.(onConstructors) as X11. red in X11.
@@ -521,19 +687,16 @@ Proof.
           simpl. intros. destruct X2 as [? ? ? ?]; unshelve econstructor; eauto.
           * apply X; eauto.
           * clear -X0 X on_cargs. revert on_cargs.
-              generalize (cshape_args cshape).
+              generalize (cshape_args y).
               induction c; simpl; auto;
               destruct a as [na [b|] ty]; simpl in *; auto;
           split; intuition eauto.
           * clear -X0 X on_cindices.
             revert on_cindices.
-            generalize (List.rev  (lift_context #|cshape_args cshape| 0 (ind_indices X1))).
-            generalize (cshape_indices cshape).
+            generalize (List.rev  (lift_context #|cshape_args y| 0 (ind_indices X1))).
+            generalize (cshape_indices y).
             induction 1; simpl; constructor; auto.
-       --- simpl; intros. pose (onProjections X1 H0). simpl in *.
-           destruct o0. constructor; auto. eapply Alli_impl; intuition eauto.
-           unfold on_projection in *; simpl in *.
-           now apply X.
+       --- simpl; intros. pose (onProjections X1 H0). simpl in *; auto.
        --- destruct X1. simpl. unfold check_ind_sorts in *.
            destruct universe_family; auto.
            split. apply ind_sorts. destruct indices_matter; auto.
@@ -548,7 +711,7 @@ Proof.
 Qed.
 
 
-Lemma declared_decl_closed `{checker_flags} (Σ : global_env) cst decl :
+Lemma declared_decl_closed `{checker_flags} {Σ : global_env} {cst decl} :
   wf Σ ->
   lookup_env Σ cst = Some decl ->
   on_global_decl (fun Σ Γ b t => closedn #|Γ| b && option_default (closedn #|Γ|) t true)
@@ -583,6 +746,89 @@ Proof.
   apply cll.
   intros. apply Hfg. simpl; lia. simpl. lia. simpl.
   eapply closed_decl_upwards; eauto. lia.
+Qed.
+
+
+Definition closed_inductive_body mdecl idecl :=
+  closedn 0 idecl.(ind_type) &&
+  forallb (fun cdecl => 
+    closedn (#|arities_context mdecl.(ind_bodies)|) (cdecl_type cdecl)) idecl.(ind_ctors) &&
+  forallb (fun x => closedn (S (ind_npars mdecl)) x.2) idecl.(ind_projs).
+
+Definition closed_inductive_decl mdecl :=
+  closed_ctx (ind_params mdecl) &&
+  forallb (closed_inductive_body mdecl) (ind_bodies mdecl). 
+  
+
+Lemma closedn_All_local_env (ctx : list context_decl) :
+  All_local_env 
+    (fun (Γ : context) (b : term) (t : option term) =>
+      closedn #|Γ| b && option_default (closedn #|Γ|) t true) ctx ->
+    closedn_ctx 0 ctx.
+Proof.
+  induction 1. constructor.
+  rewrite /closedn_ctx /= mapi_app forallb_app /= [forallb _ _]IHX /id /closed_decl /=.
+  now rewrite Nat.add_0_r List.rev_length t0.
+  rewrite /closedn_ctx /= mapi_app forallb_app /= [forallb _ _]IHX /id /closed_decl /=.
+  now rewrite Nat.add_0_r List.rev_length t1.
+Qed.
+
+Lemma skipn_0 {A} (l : list A) : skipn 0 l = l.
+Proof. reflexivity. Qed.
+
+Lemma declared_projection_closed {cf:checker_flags} {Σ : global_env_ext} {mdecl idecl p pdecl} : 
+  wf Σ.1 ->
+  declared_projection Σ.1 mdecl idecl p pdecl ->
+  closedn (S (ind_npars mdecl)) pdecl.2.
+Proof.
+  intros; eapply declared_projection_closed_ind; eauto.
+  eapply typecheck_closed; eauto. eapply type_Prop.
+Qed.
+
+Lemma declared_inductive_closed {cf:checker_flags} {Σ : global_env_ext} {mdecl mind} : 
+  wf Σ.1 ->
+  declared_minductive Σ.1 mind mdecl ->
+  closed_inductive_decl mdecl.
+Proof.
+  intros wfΣ decl.
+  pose proof (declared_decl_closed wfΣ decl) as decl'.
+  red in decl'.
+  unfold closed_inductive_decl.
+  apply andb_and. split. apply onParams in decl'.
+  now apply closedn_All_local_env in decl'; auto.
+  apply onInductives in decl'.
+  eapply All_forallb.
+  
+  assert (Alli (fun i =>  declared_inductive Σ.1 mdecl {| inductive_mind := mind; inductive_ind := i |}) 
+    0 (ind_bodies mdecl)).
+  { eapply forall_nth_error_Alli. intros.
+    split; auto. }
+  eapply Alli_mix in decl'; eauto. clear X.
+  clear decl.
+  eapply Alli_All; eauto.
+  intros n x [decli oib].
+  rewrite /closed_inductive_body.
+  apply andb_and; split. apply andb_and. split.
+  - apply onArity in oib. hnf in oib.
+    now move/andP: oib => [].
+  - pose proof (onConstructors oib).
+    red in X. eapply All_forallb. eapply All2_All_left; eauto.
+    firstorder auto.
+    eapply on_ctype in X0.
+    now move/andP: X0 => [].
+  - eapply All_forallb.
+    pose proof (onProjections oib).
+    destruct (eq_dec (ind_projs x) []) as [->|eq]; try constructor.
+    specialize (X eq). clear eq.
+    destruct (ind_cshapes oib) as [|? []]; try contradiction.
+    apply on_projs in X.
+    assert (Alli (fun i pdecl => declared_projection Σ.1 mdecl x 
+     (({| inductive_mind := mind; inductive_ind := n |}, mdecl.(ind_npars)), i) pdecl)
+      0 (ind_projs x)).
+    { eapply forall_nth_error_Alli.
+      intros. split; auto. }
+    eapply (Alli_All X0). intros.
+    now eapply declared_projection_closed in H.
 Qed.
 
 Lemma rev_subst_instance_context u Γ :
@@ -623,3 +869,5 @@ Proof.
   apply typecheck_closed in c; eauto.
   now move: c => [_ /andP [_ ct]].
 Qed.
+
+
