pcuic/theories/PCUICValidity.v
@@ -1,4 +1,4 @@
-From Coq Require Import String Bool List PeanoNat.
+From Coq Require Import String Bool List PeanoNat Lia.
 From MetaCoq.Template Require Import config utils.
 From MetaCoq.PCUIC Require Import PCUICAst
      PCUICLiftSubst PCUICTyping PCUICWeakeningEnv PCUICWeakening PCUICInversion
@@ -216,6 +216,7 @@ Section Validity.
     now eapply isWAT_it_mkProd_or_LetIn_wf_local in declm.
   Qed.
 
+
   Lemma isWfArity_or_Type_extends : forall (cf : checker_flags) (Σ : global_env)
       (Σ' : PCUICEnvironment.global_env) (φ : universes_decl),
     wf Σ' ->
@@ -236,7 +237,7 @@ Section Validity.
   Lemma weaken_env_prop_isWAT :
     weaken_env_prop
     (lift_typing
-         (fun (Σ0 : PCUICEnvironment.global_env_ext)
+        (fun (Σ0 : PCUICEnvironment.global_env_ext)
           (Γ0 : PCUICEnvironment.context) (_ T : term) =>
         isWfArity_or_Type Σ0 Γ0 T)).
   Proof.
@@ -245,6 +246,619 @@ Section Validity.
     destruct T. now eapply isWfArity_or_Type_extends.
     destruct X1 as [s Hs]; exists s; now eapply isWfArity_or_Type_extends.
   Qed.
+
+  (* Lemma type_local_ctx_smash Γ s Σ :
+    type_local_ctx
+      (lift_typing
+      (fun (Σ : PCUICEnvironment.global_env_ext) 
+          (Γ : context) (_ T : term) => isWfArity_or_Type Σ Γ T))
+    Σ Γ Δ 
+  (PCUICEnvironment.arities_context
+     (PCUICEnvironment.ind_bodies mdecl) ,,,
+   PCUICEnvironment.ind_params mdecl) (cshape_args c) 
+  (cshape_sort c) *)
+
+  Local Notation isWAT :=
+    (lift_typing
+      (fun (Σ0 : PCUICEnvironment.global_env_ext) (Γ : context) (_ T : term)
+    => isWfArity_or_Type Σ0 Γ T)).
+(* 
+  Lemma All_local_env_isWAT_wf_local Σ Γ :
+    wf_local Σ Γ ->
+    All_local_env (isWAT Σ) Γ.
+  Proof.
+    intros; eapply All_local_env_impl; eauto.
+    intros. red in X0.
+    destruct T; hnf. 2:{} *)
+
+  Lemma subst_context_smash_context s k Γ Δ :
+    subst_context s k (smash_context Γ Δ) = 
+    smash_context (subst_context s (#|Δ| + k) Γ) (subst_context s k Δ).
+  Proof.
+    induction Δ as [|[? [] ?] ?] in Γ |- *; simpl; auto;
+     rewrite subst_context_snoc; simpl.
+    - rewrite IHΔ. f_equal.
+      rewrite !subst_context_alt !mapi_mapi. apply mapi_ext. clear.
+      intros n x. rewrite /subst_decl !PCUICAstUtils.compose_map_decl.
+      eapply PCUICAstUtils.map_decl_ext. intros.
+      autorewrite with len. rewrite Nat.add_0_r.
+      generalize (Nat.pred #|Γ| - n). generalize (#|Δ| + k). clear.
+      intros. rewrite distr_subst_rec. simpl. now rewrite -Nat.add_assoc.
+    - rewrite IHΔ. f_equal.
+      rewrite subst_context_app. simpl.  unfold app_context. f_equal.
+  Qed.
+
+  Lemma wf_local_smash_context_gen Σ Γ Δ :
+    wf Σ.1 ->
+    wf_local Σ Γ -> All_local_env (fun Δ => lift_typing typing Σ (Γ ,,, Δ)) Δ -> 
+    wf_local Σ (smash_context Δ Γ).
+  Proof.
+    intros wfΣ.
+    induction 1 in Δ |- *; simpl; auto.
+    - intros wfΔ. eapply (All_local_env_impl _ _ _ wfΔ).
+      intros. now rewrite app_context_nil_l in X.
+    - intros a.
+      apply IHX. eapply All_local_env_app_inv. split; auto.
+      repeat constructor; auto.
+      eapply All_local_env_impl; eauto. simpl; intros.
+      now rewrite app_context_assoc.
+    - intros a.
+      apply IHX. eapply All_local_env_subst; eauto. simpl; intros.
+      destruct T; unfold lift_typing in *; simpl in *; firstorder auto.
+      rewrite Nat.add_0_r.
+      eapply (substitution _ Γ [vdef na b t] [b] Γ0) in X0; eauto.
+      rewrite -{1}(subst_empty 0 b). repeat constructor. now rewrite !subst_empty.
+      exists x.
+      rewrite Nat.add_0_r.
+      eapply (substitution _ Γ [vdef na b t] [b] Γ0) in p; eauto.
+      rewrite -{1}(subst_empty 0 b). repeat constructor. now rewrite !subst_empty.
+  Qed.
+  
+  Lemma wf_local_smash_context Σ Γ :
+    wf Σ.1 -> wf_local Σ Γ -> wf_local Σ (smash_context [] Γ).
+  Proof.
+    intros; eapply wf_local_smash_context_gen; eauto.
+  Qed.
+
+
+  Lemma nth_error_ass_subst_context s k Γ : 
+    (forall n d, nth_error Γ n = Some d -> decl_body d = None) ->
+    forall n d, nth_error (subst_context s k Γ) n = Some d -> decl_body d = None.
+  Proof.
+    induction Γ as [|[? [] ?] ?] in |- *; simpl; auto;
+    intros; destruct n; simpl in *; rewrite ?subst_context_snoc in H0; simpl in H0.
+    - noconf H0; simpl.
+      specialize (H 0 _ eq_refl). simpl in H; discriminate.
+    - specialize (H 0 _ eq_refl). simpl in H; discriminate.
+    - noconf H0; simpl. auto.
+    - eapply IHΓ. intros. now specialize (H (S n0) d0 H1).
+      eauto.
+  Qed.
+
+  Lemma nth_error_smash_context Γ Δ : 
+    (forall n d, nth_error Δ n = Some d -> decl_body d = None) ->
+    forall n d, nth_error (smash_context Δ Γ) n = Some d -> decl_body d = None.
+  Proof.
+    induction Γ as [|[? [] ?] ?] in Δ |- *; simpl; auto.
+    - intros. eapply (IHΓ (subst_context [t] 0 Δ)).
+      apply nth_error_ass_subst_context. auto. eauto.
+    - intros. eapply IHΓ. 2:eauto.
+      intros.
+      pose proof (nth_error_Some_length H1). autorewrite with len in H2. simpl in H2.
+      destruct (eq_dec n0 #|Δ|). subst.
+      rewrite nth_error_app_ge in H1. lia. rewrite Nat.sub_diag /= in H1. noconf H1.
+      reflexivity.
+      rewrite nth_error_app_lt in H1; try lia. eauto.
+  Qed.
+
+  Lemma fold_context_compose f g Γ : 
+    fold_context f (fold_context g Γ) = fold_context (fun n x => f n (g n x)) Γ.
+  Proof.
+    induction Γ; simpl; auto; rewrite !fold_context_snoc0.
+    simpl. rewrite IHΓ. f_equal.
+    rewrite PCUICAstUtils.compose_map_decl.
+    now rewrite fold_context_length.
+  Qed.
+
+  Lemma fold_context_ext f g Γ : 
+    f =2 g ->
+    fold_context f Γ = fold_context g Γ.
+  Proof.
+    intros hfg.
+    induction Γ; simpl; auto; rewrite !fold_context_snoc0.
+    simpl. rewrite IHΓ. f_equal. apply PCUICAstUtils.map_decl_ext.
+    intros. now apply hfg.
+  Qed.
+
+  (* Replace index k with n in i, k + S n |- x -> i, n, n, k
+  Lemma subst_under_lift s n k x i : 
+
+    subst s k (lift n (k + #|s|) x) = lift n k (subst s 0 x).
+ *)
+  Arguments Nat.sub : simpl never.
+  (* Smashing a context Γ with Δ depending on it is the same as smashing Γ
+     and substituting all references to Γ in Δ by the expansions of let bindings.
+  *)
+
+  Local Open Scope sigma.
+  Require Import PCUICSigmaCalculus PCUICClosed.
+  Lemma Upn_compose n σ σ' : ⇑^n σ ∘s ⇑^n σ' =1 ⇑^n (σ ∘s σ').
+  Proof.
+    induction n. unfold Upn. simpl.
+    now rewrite !subst_consn_nil !shiftk_0 !compose_ids_r.
+    rewrite !Upn_S. autorewrite with sigma. now rewrite IHn.
+  Qed.
+
+  Fixpoint extended_subst (Γ : context) (n : nat) :=
+    match Γ with
+    | nil => nil
+    | cons d vs =>
+      match decl_body d with
+      | Some b =>
+        (* Δ , vs |- b *)
+        let s := extended_subst vs n in
+        (* Δ , smash_context vs |- s : vs *)
+        let b' := subst0 s (lift (context_assumptions vs) #|s| b) in
+        (* Δ, smash_context vs |- b' *)
+        b' :: s
+      | None => tRel n :: extended_subst vs (S n)
+      end
+    end.
+
+  Lemma extended_subst_length Γ n : #|extended_subst Γ n| = #|Γ|.
+  Proof.
+    induction Γ in n |- *; simpl; auto.
+    now destruct a as [? [?|] ?] => /=; simpl; rewrite IHΓ. 
+  Qed.
+  Hint Rewrite extended_subst_length : len.
+  (* Lemma Up_compose σ s : ⇑ σ ∘s (s ⋅n ids) *)
+
+  Lemma extended_subst_lift (Δ : context) n : 
+    extended_subst Δ n = map (lift0 n) (extended_subst Δ 0).
+  Proof.
+    rewrite -{1}(Nat.add_0_r n).
+    generalize 0 at 1 3. revert n.
+    induction Δ.
+    simpl. auto.
+    intros n n'.
+    destruct a as [na [?|] ?]. simpl.
+    f_equal. 2:auto.
+    specialize (IHΔ n n').
+    rewrite IHΔ.
+    rewrite (distr_lift_subst _ _ n 0).
+    rewrite extended_subst_length Nat.add_0_r.
+    admit.
+    simpl. f_equal; auto. specialize (IHΔ n (S n')).
+    now rewrite -Nat.add_succ_r.
+  Admitted.
+
+  Hint Rewrite Nat.add_0_r : len.
+
+  Lemma subst_consn_lt i (s : list term) σ : 
+    i < #|s| -> 
+    ∑ x, List.nth_error s i = Some x /\ (s ⋅n σ) i = x.
+  Proof.
+    clear.
+    induction i in s |- *.
+    simpl. destruct s; simpl.
+    - lia.
+    - intros lt. exists t; simpl; auto.
+    - intros lt. destruct s; [elimtype False;inv lt|].
+      simpl in *. specialize (IHi s). forward IHi by lia.
+      destruct IHi as [? ?]; firstorder.
+  Qed.
+  
+  Lemma up_ext_closed k' k s s' :
+    (forall i, i < k' -> s i = s' i) -> 
+    forall i, i < k + k' ->
+    up k s i = up k s' i.
+  Proof.
+    unfold up. intros Hs t. elim (Nat.leb_spec k t) => H; auto.
+    intros. f_equal. apply Hs. lia.
+  Qed.
+
+  Lemma inst_ext_closed s s' k t : 
+    closedn k t -> 
+    (forall x, x < k -> s x = s' x) -> 
+    inst s t = inst s' t.
+  Proof.
+    clear.
+    intros clt Hs. revert k clt s s' Hs.
+    elim t using PCUICInduction.term_forall_list_ind; simpl in |- *; intros; try easy ;
+      try (try rewrite H; try rewrite H0 ; try rewrite H1 ; easy);
+      try solve [f_equal; solve_all].
+    - apply Hs. now eapply Nat.ltb_lt. 
+    - move/andP: clt => []. intros. f_equal; eauto.
+      eapply H0; eauto. intros. eapply up_ext_closed; eauto.
+    - move/andP: clt => []. intros. f_equal; eauto. now eapply H0, up_ext_closed.
+    - move/andP: clt => [] /andP[] ?. intros. f_equal; eauto.
+      now eapply H1, up_ext_closed.
+    - move/andP: clt => [] ? ?. f_equal; eauto.
+    - move/andP: clt => [] /andP[] ? ? b1.
+      red in X. solve_all. f_equal; eauto.
+      eapply All_map_eq. eapply (All_impl b1). firstorder.
+    - f_equal; eauto. red in X. solve_all.
+      move/andP: b => []. eauto. intros.
+      apply map_def_eq_spec; eauto.
+      eapply b0; eauto. now apply up_ext_closed.
+    - f_equal; eauto. red in X. solve_all.
+      move/andP: b => []. eauto. intros.
+      apply map_def_eq_spec; eauto.
+      eapply b0; eauto. now apply up_ext_closed.
+  Qed.
+
+  Lemma subst_consn_eq s0 s1 s2 s3 x : 
+    x < #|s0| -> #|s0| = #|s2| ->
+    subst_fn s0 x = subst_fn s2 x ->
+    (s0 ⋅n s1) x = (s2 ⋅n s3) x.
+  Proof.
+    unfold subst_fn; intros Hx Heq Heqx.
+    unfold subst_consn. 
+    destruct (nth_error s0 x) eqn:Heq';
+    destruct (nth_error s2 x) eqn:Heq''; auto.
+    apply nth_error_None in Heq''. lia.
+    apply nth_error_None in Heq'. lia.
+    apply nth_error_None in Heq'. lia.
+  Qed.
+
+  Lemma inst_extended_subst_shift_ind (Γ : context) k : 
+    closed_ctx Γ ->
+    (forall x, x < #|Γ| -> 
+      option_map (fun x0 : term => x0.[↑^k]) (nth_error (extended_subst Γ 0) x) =
+      nth_error (extended_subst Γ k) x) ->
+    map (inst ((extended_subst Γ 0 ⋅n ids) ∘s ↑^k)) (idsn #|Γ|) =
+    map (inst (extended_subst Γ k ⋅n ids)) (idsn #|Γ|).
+  Proof.
+    intros.
+    rewrite !map_idsn_spec.
+    apply nat_recursion_ext => x l' Hx.
+    f_equal. f_equal.
+    edestruct (subst_consn_lt x (extended_subst Γ k) ids) as [d [Hd Hσ]].
+    now (autorewrite with len; lia).
+    simpl. rewrite Hσ.
+    edestruct (subst_consn_lt x (extended_subst Γ 0) ids) as [d' [Hd' Hσ']].
+    now autorewrite with len.
+    unfold subst_compose. rewrite Hσ'.
+    apply some_inj.
+    rewrite -Hd. change (Some d'.[↑^k]) with (option_map (fun x => inst (↑^k) x) (Some d')).
+    rewrite -Hd'. now apply H0.
+  Qed.
+
+  Hint Rewrite idsn_length : len.
+
+  Lemma subst_fn_eq s s' x : s = s' -> subst_fn s x = subst_fn s' x.
+  Proof.
+    intros -> ; reflexivity.
+  Qed.
+
+  Lemma extended_subst_shift (Γ : context) k : 
+    closed_ctx Γ ->
+    forall x, x < #|Γ| -> 
+    option_map (fun x0 : term => x0.[↑^k]) (nth_error (extended_subst Γ 0) x) =
+    nth_error (extended_subst Γ k) x.
+  Proof.
+    intros clΓ.
+    induction Γ in k, clΓ |- *. simpl. lia.
+    simpl; intros x Hx.
+    intros. 
+    destruct a as [? [] ?]; auto.
+    simpl.
+    autorewrite with sigma.
+    rewrite !ren_lift_renaming. autorewrite with len.
+    rewrite Upn_eq. rewrite !subst_consn_compose.
+    autorewrite with sigma.
+    move/closedn_ctx_cons/andP: clΓ => [clΓ /andP [clt _]].
+    simpl in clt.
+    destruct x. simpl. f_equal.
+    autorewrite with sigma.
+    rewrite subst_consn_compose.
+    eapply inst_ext_closed; eauto.
+    intros.
+    apply subst_consn_eq; autorewrite with len; auto.
+    pose proof (inst_extended_subst_shift_ind Γ k clΓ).
+    rewrite -H0. intros. apply IHΓ; auto.
+    rewrite map_map_compose. apply subst_fn_eq.
+    apply map_ext. intros.
+    now autorewrite with sigma.
+
+    simpl. apply IHΓ; auto. lia.
+
+    simpl.
+    destruct x; simpl. unfold shiftk.
+    now rewrite Nat.add_0_r.
+    move/closedn_ctx_cons/andP: clΓ => [clΓ /andP [clt _]].
+    rewrite -(IHΓ (S k)); auto. lia.
+    rewrite -(IHΓ 1 clΓ x ltac:(lia)).
+    rewrite option_map_two. apply option_map_ext.
+    intros. autorewrite with sigma.
+    now rewrite -shiftk_shift -shiftk_shift_l.
+  Qed.
+
+  Lemma inst_extended_subst_shift (Γ : context) k : 
+    closed_ctx Γ ->
+    map (inst ((extended_subst Γ 0 ⋅n ids) ∘s ↑^k)) (idsn #|Γ|) =
+    map (inst (extended_subst Γ k ⋅n ids)) (idsn #|Γ|).
+  Proof.
+    intros. apply inst_extended_subst_shift_ind; auto.
+    now apply extended_subst_shift.
+  Qed.
+
+  Lemma smash_context_acc Γ Δ : 
+    closed_ctx Γ ->
+    smash_context Δ Γ =
+        subst_context (extended_subst Γ 0) 0 (lift_context (context_assumptions Γ) #|Γ| Δ)
+     ++ smash_context [] Γ.
+  Proof.
+    revert Δ.
+    induction Γ as [|[? [] ?] ?]; intros Δ cl.
+    - simpl; auto.
+      now rewrite subst0_context app_nil_r lift0_context.
+    - simpl. autorewrite with len.
+      move/closedn_ctx_cons/andP: cl => [clΓ /andP [clt _]].
+      rewrite IHΓ; auto.
+      rewrite subst_context_nil. f_equal.
+      rewrite (subst_context_decompo [_] _).
+      simpl. autorewrite with len.
+      rewrite lift0_id.
+      rewrite subst0_context.
+      unfold subst_context, lift_context.
+      rewrite !fold_context_compose.
+      apply fold_context_ext. intros n n' -> x.
+      rewrite Nat.add_0_r.
+      autorewrite with sigma.
+      apply inst_ext.
+      setoid_rewrite ren_lift_renaming.
+      autorewrite with sigma.
+      rewrite !Upn_compose.
+      apply Upn_ext. 
+      autorewrite with sigma.
+      unfold Up.
+      rewrite subst_consn_subst_cons.
+      autorewrite with sigma.
+      reflexivity.
+      
+    - simpl.
+      move/closedn_ctx_cons/andP: cl => [clΓ /andP [clt _]].
+      rewrite IHΓ /=. auto.
+      rewrite (IHΓ [_]). auto. rewrite !app_assoc. f_equal.
+      rewrite app_nil_r. unfold map_decl. simpl. unfold app_context.
+      simpl. rewrite lift_context_app subst_context_app /app_context. simpl.
+      unfold lift_context at 2. unfold subst_context at 2, fold_context. simpl.
+      f_equal.
+      unfold subst_context, lift_context.
+      rewrite !fold_context_compose.
+      apply fold_context_ext. intros n n' ->. intros x.
+      rewrite Nat.add_0_r.
+
+      autorewrite with sigma.
+      apply inst_ext. rewrite !ren_lift_renaming.
+      autorewrite with sigma.
+      rewrite !Upn_compose.
+      autorewrite with sigma.
+      apply Upn_ext.
+      unfold Up.
+      
+      rewrite subst_consn_subst_cons.
+      autorewrite with sigma.
+      apply subst_cons_proper. auto.
+      rewrite !Upn_eq. autorewrite with sigma.
+      rewrite !subst_consn_compose.
+      setoid_rewrite subst_consn_compose at 2 3.
+      apply subst_consn_proper.
+      rewrite -inst_extended_subst_shift; auto.
+
+      autorewrite with sigma.
+      rewrite -subst_compose_assoc.
+      rewrite shiftk_compose.
+      autorewrite with sigma.
+      setoid_rewrite <- (compose_ids_l ↑) at 2.
+      rewrite -subst_consn_compose.
+      rewrite - !subst_compose_assoc.
+      rewrite -shiftk_shift shiftk_compose.
+      autorewrite with sigma.
+      rewrite subst_consn_compose.
+      rewrite -shiftk_compose subst_compose_assoc.
+      rewrite subst_consn_shiftn.
+      2:now autorewrite with len.
+      autorewrite with sigma. 
+      rewrite -shiftk_shift.
+      rewrite -shiftk_compose subst_compose_assoc.
+      rewrite subst_consn_shiftn.
+      2:now autorewrite with len.
+      now autorewrite with sigma.
+  Qed.
+
+  Lemma skipn_0_eq {A} (l : list A) n : n =  0 -> skipn n l = l.
+  Proof. intros ->; apply PCUICAstUtils.skipn_0. Qed.
+ 
+  Lemma extended_subst_to_extended_list_k Γ k :
+    (map (subst0 (extended_subst Γ k)) (to_extended_list_k Γ k)) = 
+    to_extended_list_k (smash_context [] Γ) k.
+  Proof.
+    induction Γ in k |- *. simpl. reflexivity.
+    unfold to_extended_list_k. simpl.
+    destruct a as [? [] ?]; simpl. admit.
+  Admitted.
+
+
+  (* Well, it's a smash_context mess! *)
+  Lemma declared_projection {Σ : global_env_ext} {mdecl idecl p pdecl} : 
+    wf Σ.1 ->
+    declared_projection Σ.1 mdecl idecl p pdecl ->
+    let u := PCUICLookup.abstract_instance (ind_universes mdecl) in
+    let ind := p.1.1 in
+    isType (Σ.1, ind_universes mdecl)
+      ((vass nAnon (mkApps (tInd ind u) (to_extended_list (smash_context [] (ind_params mdecl)))))::
+         smash_context [] (ind_params mdecl)) pdecl.2.
+  Proof.
+    intros wfΣ isdecl u ind.
+    destruct (on_declared_projection wfΣ isdecl) as [oni onp].
+    set (declared_inductive_inv _ wfΣ _ isdecl.p1) as oib in *.
+    clearbody oib.
+    have onpars := onParams _ _ _ _ (declared_minductive_inv weaken_env_prop_typing wfΣ wfΣ isdecl.p1.p1).
+    have parslen := onNpars _ _ _ _ (declared_minductive_inv weaken_env_prop_typing wfΣ wfΣ isdecl.p1.p1).
+    simpl in onp. destruct (ind_cshapes oib) as [|? []] eqn:Heq; try contradiction.
+    red in onp.
+    destruct (nth_error (smash_context [] _) _) eqn:Heq'; try contradiction.
+    rewrite {}onp.
+    assert(onProjs :  on_projections mdecl (inductive_mind p.1.1) (inductive_ind p.1.1) idecl (ind_indices oib) c).
+    { destruct oib.
+      assert (ind_projs idecl <> []).
+      { destruct isdecl as [? [hnth]]. eapply nth_error_Some_non_nil in hnth; auto. }
+      simpl in Heq. simpl. rewrite Heq in onProjections.
+      now specialize (onProjections H). }
+    assert(projslen : #|ind_projs idecl| = (context_assumptions (cshape_args c))).
+    { now destruct onProjs. }
+    assert (some_proj :#|ind_projs idecl| > 0).
+    { destruct isdecl as [ [] []]. now apply nth_error_Some_length in H1. }
+    pose proof (onConstructors oib) as onc. 
+    red in onc. rewrite Heq in onc. inv onc. clear X0.
+    eapply on_cargs in X.
+    simpl.
+    assert (wf_local (Σ.1, ind_universes mdecl) (arities_context (ind_bodies mdecl))).
+    { eapply wf_arities_context; eauto. now destruct isdecl as [[] ?]. }
+    eapply PCUICClosed.type_local_ctx_All_local_env in X.
+    2:{ eapply All_local_env_app_inv. split; auto.
+        red in onpars. eapply (All_local_env_impl _ _ _ onpars).
+        intros. destruct T; simpl in *.
+        - eapply weaken_ctx; auto.
+        - destruct X1 as [s Hs]. exists s. apply weaken_ctx; auto. }
+    rewrite -(app_context_nil_l (arities_context _)) in X.
+    rewrite -app_context_assoc in X.
+    eapply (substitution_wf_local _ []) in X; auto.
+    2:{ eapply subslet_inds_gen; eauto. destruct isdecl as []; eauto. }
+    rewrite app_context_nil_l in X.
+    epose proof (nth_error_subst_context _ _ _ _).
+    erewrite Heq' in H. autorewrite with len in H. clear Heq'.
+    rewrite subst_context_smash_context in H.
+    autorewrite with len in H. rewrite subst_context_nil in H.
+    move: X.
+    rewrite subst_context_app.
+    rewrite (closed_ctx_subst _ _ (ind_params mdecl)).
+    red in onpars. eapply closed_wf_local; [|eauto]. auto.
+    assert (parsu : subst_instance_context u (ind_params mdecl) = ind_params mdecl). admit.
+    assert (sortu : subst_instance_univ u (ind_sort oib) = ind_sort oib). admit.
+    pose proof (spine_subst_to_extended_list_k (Σ.1, ind_universes mdecl)
+      (ind_params mdecl) []).
+    forward X; auto.
+    forward X. rewrite app_context_nil_l; auto.
+    rewrite app_context_nil_l in X.
+    rewrite closed_ctx_lift in X.
+    red in onpars. eapply closed_wf_local; [|eauto]. auto.
+    assert(wf_local (Σ.1, ind_universes mdecl) (ind_params mdecl ,, vass nAnon (mkApps (tInd ind u) (to_extended_list (ind_params mdecl))))).
+    constructor. auto. red. exists (ind_sort oib).
+    eapply type_mkApps. econstructor; eauto.
+    destruct isdecl as []; eauto. subst u. admit.
+    rewrite (ind_arity_eq oib).
+    rewrite subst_instance_constr_it_mkProd_or_LetIn.
+    rewrite -(app_nil_r (to_extended_list _)).
+    eapply typing_spine_it_mkProd_or_LetIn'; auto.
+    rewrite parsu. eapply X.
+    constructor. left. eexists _, _; simpl; intuition auto.
+    pose proof (onProjs.(on_projs_noidx _ _ _ _ _ _)).
+    destruct (ind_indices oib); simpl in H0; try discriminate.
+    simpl. rewrite sortu. reflexivity.
+    rewrite -subst_instance_constr_it_mkProd_or_LetIn.
+    right. pose proof (onArity oib). rewrite -(oib.(ind_arity_eq)).
+    destruct X1 as [s Hs]. exists s.
+    eapply (weaken_ctx (Γ:=[])). auto. auto. admit.
+    intros wf.
+    generalize (weakening_wf_local _ _ _ [_] _ wf X1).
+    simpl; clear X1 wf.
+    move/wf_local_smash_context => /=.
+    rewrite smash_context_app /= smash_context_acc.
+    red in onpars. eapply closed_wf_local; [|eauto]. auto.
+    set(indsubst := (inds (inductive_mind p.1.1) (PCUICLookup.abstract_instance (PCUICEnvironment.ind_universes mdecl))
+      (PCUICEnvironment.ind_bodies mdecl))) in *.
+    set (projsubst :=  (projs {| inductive_mind := inductive_mind p.1.1; inductive_ind := inductive_ind p.1.1 |}
+    (PCUICEnvironment.ind_npars mdecl) p.2)) in *.
+    rewrite lift_context_app. simpl.
+    rewrite [subst_context _ _ (_ ++ _)]subst_context_app.
+    simpl. unfold app_context. simpl.
+    unfold lift_context at 3. unfold fold_context. simpl.
+    unfold map_decl. simpl. rewrite lift_mkApps. simpl.
+    rewrite {3}/subst_context /fold_context /= /map_decl /= subst_mkApps /=.
+    rewrite /to_extended_list lift_to_extended_list_k.
+    rewrite extended_subst_to_extended_list_k.
+    fold (to_extended_list (smash_context [] (ind_params mdecl))).
+    intros wfl.
+    rewrite PCUICClosed.closed_ctx_lift in wfl. admit.
+    
+
+
+    rewrite -reln_lift.
+    set(foo:= subst_context _ _ _).
+    rewrite subst_context_app.
+    eapply nth_error_All_local_env in X.
+    2:{ eapply nth_error_Some_length in H. apply H. }
+    unfold app_context in X. erewrite H in X.
+    simpl in X, H. red in X.
+    destruct c0 as [? [] ?]; simpl in *.
+    unfold subst_decl, map_decl in H; simpl in H.
+    eapply nth_error_smash_context in H. simpl in H. discriminate.
+    clear H.
+    intros. rewrite nth_error_nil // in H.
+    destruct X as [s Hs].
+    rewrite smash_context_length /= in Hs.
+    rewrite PCUICClosed.context_assumptions_app Nat.add_0_r in Hs.
+    clear H.
+    set (k := context_assumptions (cshape_args c) - p.2) in *.
+    rewrite subst_context_app Nat.add_0_r in Hs.
+    rewrite (closed_ctx_subst _ _ (ind_params mdecl)) in Hs.
+    red in onpars. eapply closed_wf_local; [|eauto]. auto.
+    rewrite /app_context smash_context_app in Hs.
+    exists s. red.
+    rewrite smash_context_acc in Hs.
+    rewrite skipn_app in Hs.
+    autorewrite with len in Hs. rewrite !smash_context_length in Hs.
+    rewrite context_assumptions_fold in Hs.
+    rewrite (skipn_0_eq _ (S _ - _)) in Hs.
+    simpl length. lia.
+    destruct isdecl as [? []]. apply nth_error_Some_length in H0.
+    rewrite projslen in H0. rewrite projslen in some_proj. lia.
+    simpl. lia.
+
+
+    
+
+
+
+    replace ((context_assumptions (cshape_args c) +
+    context_assumptions (PCUICEnvironment.ind_params mdecl) -
+    S (PCUICEnvironment.context_assumptions (cshape_args c) - p.2)))
+    with  (context_assumptions (PCUICEnvironment.ind_params mdecl) + S p.2) by lia.
+        S (PCUICEnvironment.context_assumptions (cshape_args c) - p.2)))
+    autorewrite with len in Hs.
+
+    eexists _.
+    rename X into args.
+    apply type_local_ctx_Pclosed in args.
+    red in onpars.
+    eapply All_local_env_Pclosed in onpars.
+    eapply (Alli_impl (Q:=fun i d => closed_decl (#|ind_params mdecl| + i + #|arities_context (ind_bodies mdecl)|) d)) in args.
+    2:{ intros n x. rewrite app_context_length. 
+        intros H; eapply closed_decl_upwards; eauto. lia. }
+    eapply (Alli_shiftn (P:=fun i d => closed_decl (i + #|arities_context (ind_bodies mdecl)|) d)) in args.
+    rewrite Nat.add_0_r in args.
+    eapply (Alli_impl (Q:=fun i d => closed_decl (i + #|arities_context (ind_bodies mdecl)|) d)) in onpars.
+    2:{ intros n x d. eapply closed_decl_upwards; eauto; lia. }
+    epose proof (Alli_app_inv onpars). rewrite List.rev_length /= in X.
+    specialize (X args). rewrite -List.rev_app_distr in X.
+    clear onpars args.
+    eapply (Alli_impl (Q:=fun i d => closed_decl (#|arities_context (ind_bodies mdecl)| + i) d)) in X.
+    2:intros; eapply closed_decl_upwards; eauto; lia.
+    eapply closed_smash_context in X.
+    eapply Alli_rev_nth_error in X; eauto.
+    rewrite smash_context_length in X. simpl in X.
+    eapply nth_error_Some_length in Heq'. rewrite smash_context_length in Heq'.
+    simpl in Heq'. unfold closed_decl in X.
+    move/andP: X => [] _ cl.
+    eapply closed_upwards. eauto. rewrite arities_context_length.
+    rewrite context_assumptions_app parslen.
+    rewrite context_assumptions_app in Heq'. lia.
+  Qed.
+ *)
+
 
   Theorem validity :
     env_prop (fun Σ Γ t T => isWfArity_or_Type Σ Γ T)
@@ -371,13 +985,13 @@ Section Validity.
       right; simpl; apply o0.
 
     - (* Constant type *)
-      destruct (on_declared_constructor wf isdecl) as [[oni oib] [s [decli [cs onc]]]].
+      destruct (on_declared_constructor wf isdecl) as [[oni oib] [cs [declc onc]]].
       unfold type_of_constructor.
-      right. red in onc. red in onc.
-      destruct onc as [s' Hs].
+      right. have ctype := on_ctype onc.
+      destruct ctype as [s' Hs].
       exists (subst_instance_univ u s').
       eapply instantiate_minductive in Hs; eauto.
-      2:(destruct isdecl as [[] _]; eauto).
+      2:(destruct isdecl as [[] ?]; eauto).
       simpl in Hs.
       eapply (weaken_ctx (Γ:=[]) Γ); eauto.
       eapply (substitution _ [] _ (inds _ _ _) [] _ (tSort _)); eauto.
@@ -416,7 +1030,9 @@ Section Validity.
 
     - (* Proj *)
       right.
-      apply on_declared_projection in isdecl as [[onm oni] onp]=> //.
+      destruct (on_declared_projection wf isdecl) as [oni onp].
+      destruct declared_inductive_inv. simpl in onp.
+      as [[onm oni] onp]=> //.
       destruct onp as [s Hty].
       exists s.
       subst ty.
