pcuic/theories/PCUICSR.v
@@ -1875,8 +1875,7 @@ Definition sr_stmt {cf:checker_flags} (Σ : global_env_ext) Γ t T :=
   forall u, red Σ Γ t u -> Σ ;;; Γ |- u : T.
 
 Theorem subject_reduction {cf:checker_flags} : 
-   forall (Σ : global_env_ext) Γ t u T,
-  wf Σ -> Σ ;;; Γ |- t : T -> red Σ Γ t u -> Σ ;;; Γ |- u : T.
+  forall (Σ : global_env_ext) Γ t u T, wf Σ -> Σ ;;; Γ |- t : T -> red Σ Γ t u -> Σ ;;; Γ |- u : T.
 Proof.
   intros * wfΣ Hty Hred.
   induction Hred. auto.
